### Solution

Based on the formula for the sum of cubes $a^3 + b^3 = (a + b)(a^2 − ab + b^2)$, we can factorize the left side:

$$(x − 7)^3 + (x + 3)^3 = 278(x − 2)$$

$$(2x − 4)((x − 7)^2 − (x − 7)(x + 3) + (x + 3)^2) = 278(x − 2)$$

One solution is obviously $x_1 = 2$.  
The other solutions are obtained by removing $2(x − 2)$ from both sides, on the left side we then have:

$$(x^2 − 14x + 49) − (x^2 − 4x − 21) + (x^2 + 6x + 9) = 139$$

$$x^2 − 4x + 79 = 139$$

Solving the quadratic equation we get the remaining two solutions:

$$x_{2/3} = \frac{4 \pm \sqrt{16 + 240}}{2}$$

$$x_{2/3} = \frac{4 \pm 16}{2}$$

$$x_2 = -6$$

$$x_3 = 10$$